removing MasterSecret from tls-gen temporarily ... some extraction bug

src/tls/ConnInvariant.fst
@@ -56,16 +56,6 @@ let ms_conn_invariant (ms:ms_tab)
  		      (conn:c_tab)
 		      (h:HyperHeap.t) 
   = forall (i:id) .{:pattern (MM.sel ms i)} ms_conn_inv ms conn h i
-  
-	     (* authId i /\ StAE.is_stream_ae i ==>  //Focused only on TLS-1.3 for now, hence the is_stream_ae guard *)
-	     (*        (match MM.sel ms i with  *)
-	     (* 	     | None -> True *)
-	     (* 	     | Some w ->  *)
-	     (* 	       Map.contains h (StreamAE.State.region w) /\ //technical for framing; need to know that the writer's region exists *)
- 	     (* 	       (MR.m_sel h (StreamAE.ilog (StreamAE.State.log w)) = Seq.createEmpty  \/   //the writer is still unused; or *)
-	     (* 	        False)) *)
-	     (* 	        (\* (let copt = MM.sel conn (I.nonce_of_id i) in *\) *)
-  	     (* 		(\*  is_Some copt /\ registered i w (Some.v copt) h)))      //it's been assigned to a connection *\) *)
 
 let mc_inv (h:HyperHeap.t) = ms_conn_invariant (MR.m_sel h MS.ms_tab) (MR.m_sel h conn_table) h
 
@@ -73,8 +63,7 @@ let mc_inv (h:HyperHeap.t) = ms_conn_invariant (MR.m_sel h MS.ms_tab) (MR.m_sel 
 
 //1. Deriving a new key involves adding a new writer to the ms table (because we tried a lookup at id and it failed)
 //   Easy: because a new log is empty and both cases of the conn table allow empty logs to be in ms
-
-val ms_derive_is_ok': h0:HyperHeap.t -> h1:HyperHeap.t -> i:id -> w:MS.writer i -> j:id
+val ms_derive_is_ok: h0:HyperHeap.t -> h1:HyperHeap.t -> i:id -> w:MS.writer i 
   -> Lemma (requires 
 		 HH.contains_ref (MR.as_rref conn_table) h0 /\
 		 HH.contains_ref (MR.as_rref MS.ms_tab) h0 /\
@@ -90,25 +79,26 @@ val ms_derive_is_ok': h0:HyperHeap.t -> h1:HyperHeap.t -> i:id -> w:MS.writer i 
 		  MM.sel old_ms i = None /\
 		  new_ms = MM.upd old_ms i w) /\                                    //and the ms_tab only changed by adding w
 		 MR.m_sel h1 (StreamAE.ilog (StreamAE.State.log w)) = Seq.createEmpty)             //and w's log is empty
-	 (ensures (
-		  let new_ms = MR.m_sel h1 MS.ms_tab in
-		  let new_conn = MR.m_sel h1 conn_table in
-		  ms_conn_inv new_ms new_conn h1 j))
-	 (* mc_inv h1)                                                       //we're back in the invariant *)
-let ms_derive_is_ok' h0 h1 i w j = 
-  let old_ms = MR.m_sel h0 MS.ms_tab in 
-  let new_ms = MR.m_sel h1 MS.ms_tab in
-  let new_conn = MR.m_sel h1 conn_table in
-  assert (ms_conn_inv new_ms new_conn h1 i);
-  if (authId j && StAE.is_stream_ae j)
-  then match MM.sel new_ms j with 
-       | None -> ()
-       | Some ww -> 
-	 if ww=w 
-	 then ()
-	 else assert (Some ww=MM.sel old_ms j)
-  else ()
-
+	 (ensures (mc_inv h1))
+let ms_derive_is_ok h0 h1 i w = 
+  let aux :  j:id -> Lemma (let new_ms = MR.m_sel h1 MS.ms_tab in
+			  let new_conn = MR.m_sel h1 conn_table in
+			  ms_conn_inv new_ms new_conn h1 j) =
+    fun j -> 			    
+      let old_ms = MR.m_sel h0 MS.ms_tab in 
+      let new_ms = MR.m_sel h1 MS.ms_tab in
+      let new_conn = MR.m_sel h1 conn_table in
+      assert (ms_conn_inv new_ms new_conn h1 i);
+      if (authId j && StAE.is_stream_ae j)
+      then match MM.sel new_ms j with 
+           | None -> ()
+           | Some ww -> 
+     	     if ww=w 
+	     then ()
+	     else assert (Some ww=MM.sel old_ms j)
+      else () in
+  qintro aux
+  
 
 (* //2. Adding a new epoch to a connection c, with a fresh index (hdId i) for c *)
 (* //      -- we found a writer w at (ms i), pre-allocated (we're second) or not (we're first) *)
